case-studies/kathrin/coq-submission/Chapter6/variadic_fin.v
@@ -1,0 +1,507 @@
+Require Export fintype.
+Require Export header_extensible.
+Inductive tm (n_tm : nat) : Type :=
+  | var_tm : forall _ : fin n_tm, tm n_tm
+  | app :
+      forall p : nat,
+      forall _ : tm n_tm, forall _ : cod (fin p) (tm n_tm), tm n_tm
+  | lam : forall p : nat, forall _ : tm (plus p n_tm), tm n_tm.
+Lemma congr_app {p : nat} {m_tm : nat} {s0 : tm m_tm}
+  {s1 : cod (fin p) (tm m_tm)} {t0 : tm m_tm} {t1 : cod (fin p) (tm m_tm)}
+  (H0 : eq s0 t0) (H1 : eq s1 t1) : eq (app m_tm p s0 s1) (app m_tm p t0 t1).
+Proof.
+exact (eq_trans (eq_trans eq_refl (ap (fun x => app m_tm p x s1) H0))
+                (ap (fun x => app m_tm p t0 x) H1)).
+Qed.
+Lemma congr_lam {p : nat} {m_tm : nat} {s0 : tm (plus p m_tm)}
+  {t0 : tm (plus p m_tm)} (H0 : eq s0 t0) :
+  eq (lam m_tm p s0) (lam m_tm p t0).
+Proof.
+exact (eq_trans eq_refl (ap (fun x => lam m_tm p x) H0)).
+Qed.
+Definition upRen_tm_tm {m : nat} {n : nat} (xi : forall _ : fin m, fin n) :
+  forall _ : fin (S m), fin (S n) := up_ren xi.
+Definition upRen_list_tm_tm (p : nat) {m : nat} {n : nat}
+  (xi : forall _ : fin m, fin n) :
+  forall _ : fin (plus p m), fin (plus p n) := upRen_p p xi.
+Fixpoint ren_tm {m_tm : nat} {n_tm : nat}
+(xi_tm : forall _ : fin m_tm, fin n_tm) (s : tm m_tm) : tm n_tm :=
+  match s with
+  | var_tm _ s0 => var_tm n_tm (xi_tm s0)
+  | app _ p s0 s1 => app n_tm p (ren_tm xi_tm s0) (cod_map (ren_tm xi_tm) s1)
+  | lam _ p s0 => lam n_tm p (ren_tm (upRen_list_tm_tm p xi_tm) s0)
+  end.
+Definition up_tm_tm {m : nat} {n_tm : nat}
+  (sigma : forall _ : fin m, tm n_tm) : forall _ : fin (S m), tm (S n_tm) :=
+  scons (var_tm (S n_tm) var_zero) (funcomp (ren_tm shift) sigma).
+Definition up_list_tm_tm (p : nat) {m : nat} {n_tm : nat}
+  (sigma : forall _ : fin m, tm n_tm) :
+  forall _ : fin (plus p m), tm (plus p n_tm) :=
+  scons_p p (funcomp (var_tm (plus p n_tm)) (zero_p p))
+    (funcomp (ren_tm (shift_p p)) sigma).
+Fixpoint subst_tm {m_tm : nat} {n_tm : nat}
+(sigma_tm : forall _ : fin m_tm, tm n_tm) (s : tm m_tm) : tm n_tm :=
+  match s with
+  | var_tm _ s0 => sigma_tm s0
+  | app _ p s0 s1 =>
+      app n_tm p (subst_tm sigma_tm s0) (cod_map (subst_tm sigma_tm) s1)
+  | lam _ p s0 => lam n_tm p (subst_tm (up_list_tm_tm p sigma_tm) s0)
+  end.
+Definition upId_tm_tm {m_tm : nat} (sigma : forall _ : fin m_tm, tm m_tm)
+  (Eq : forall x, eq (sigma x) (var_tm m_tm x)) :
+  forall x, eq (up_tm_tm sigma x) (var_tm (S m_tm) x) :=
+  fun n =>
+  match n with
+  | Some fin_n => ap (ren_tm shift) (Eq fin_n)
+  | None => eq_refl
+  end.
+Definition upId_list_tm_tm {p : nat} {m_tm : nat}
+  (sigma : forall _ : fin m_tm, tm m_tm)
+  (Eq : forall x, eq (sigma x) (var_tm m_tm x)) :
+  forall x, eq (up_list_tm_tm p sigma x) (var_tm (plus p m_tm) x) :=
+  fun n =>
+  scons_p_eta (var_tm (plus p m_tm))
+    (fun n => ap (ren_tm (shift_p p)) (Eq n)) (fun n => eq_refl).
+Fixpoint idSubst_tm {m_tm : nat} (sigma_tm : forall _ : fin m_tm, tm m_tm)
+(Eq_tm : forall x, eq (sigma_tm x) (var_tm m_tm x)) (s : tm m_tm) :
+eq (subst_tm sigma_tm s) s :=
+  match s with
+  | var_tm _ s0 => Eq_tm s0
+  | app _ p s0 s1 =>
+      congr_app (idSubst_tm sigma_tm Eq_tm s0)
+        (cod_id (idSubst_tm sigma_tm Eq_tm) s1)
+  | lam _ p s0 =>
+      congr_lam
+        (idSubst_tm (up_list_tm_tm p sigma_tm) (upId_list_tm_tm _ Eq_tm) s0)
+  end.
+Definition upExtRen_tm_tm {m : nat} {n : nat} (xi : forall _ : fin m, fin n)
+  (zeta : forall _ : fin m, fin n) (Eq : forall x, eq (xi x) (zeta x)) :
+  forall x, eq (upRen_tm_tm xi x) (upRen_tm_tm zeta x) :=
+  fun n =>
+  match n with
+  | Some fin_n => ap shift (Eq fin_n)
+  | None => eq_refl
+  end.
+Definition upExtRen_list_tm_tm {p : nat} {m : nat} {n : nat}
+  (xi : forall _ : fin m, fin n) (zeta : forall _ : fin m, fin n)
+  (Eq : forall x, eq (xi x) (zeta x)) :
+  forall x, eq (upRen_list_tm_tm p xi x) (upRen_list_tm_tm p zeta x) :=
+  fun n => scons_p_congr (fun n => eq_refl) (fun n => ap (shift_p p) (Eq n)).
+Fixpoint extRen_tm {m_tm : nat} {n_tm : nat}
+(xi_tm : forall _ : fin m_tm, fin n_tm)
+(zeta_tm : forall _ : fin m_tm, fin n_tm)
+(Eq_tm : forall x, eq (xi_tm x) (zeta_tm x)) (s : tm m_tm) :
+eq (ren_tm xi_tm s) (ren_tm zeta_tm s) :=
+  match s with
+  | var_tm _ s0 => ap (var_tm n_tm) (Eq_tm s0)
+  | app _ p s0 s1 =>
+      congr_app (extRen_tm xi_tm zeta_tm Eq_tm s0)
+        (cod_ext (extRen_tm xi_tm zeta_tm Eq_tm) s1)
+  | lam _ p s0 =>
+      congr_lam
+        (extRen_tm (upRen_list_tm_tm p xi_tm) (upRen_list_tm_tm p zeta_tm)
+           (upExtRen_list_tm_tm _ _ Eq_tm) s0)
+  end.
+Definition upExt_tm_tm {m : nat} {n_tm : nat}
+  (sigma : forall _ : fin m, tm n_tm) (tau : forall _ : fin m, tm n_tm)
+  (Eq : forall x, eq (sigma x) (tau x)) :
+  forall x, eq (up_tm_tm sigma x) (up_tm_tm tau x) :=
+  fun n =>
+  match n with
+  | Some fin_n => ap (ren_tm shift) (Eq fin_n)
+  | None => eq_refl
+  end.
+Definition upExt_list_tm_tm {p : nat} {m : nat} {n_tm : nat}
+  (sigma : forall _ : fin m, tm n_tm) (tau : forall _ : fin m, tm n_tm)
+  (Eq : forall x, eq (sigma x) (tau x)) :
+  forall x, eq (up_list_tm_tm p sigma x) (up_list_tm_tm p tau x) :=
+  fun n =>
+  scons_p_congr (fun n => eq_refl) (fun n => ap (ren_tm (shift_p p)) (Eq n)).
+Fixpoint ext_tm {m_tm : nat} {n_tm : nat}
+(sigma_tm : forall _ : fin m_tm, tm n_tm)
+(tau_tm : forall _ : fin m_tm, tm n_tm)
+(Eq_tm : forall x, eq (sigma_tm x) (tau_tm x)) (s : tm m_tm) :
+eq (subst_tm sigma_tm s) (subst_tm tau_tm s) :=
+  match s with
+  | var_tm _ s0 => Eq_tm s0
+  | app _ p s0 s1 =>
+      congr_app (ext_tm sigma_tm tau_tm Eq_tm s0)
+        (cod_ext (ext_tm sigma_tm tau_tm Eq_tm) s1)
+  | lam _ p s0 =>
+      congr_lam
+        (ext_tm (up_list_tm_tm p sigma_tm) (up_list_tm_tm p tau_tm)
+           (upExt_list_tm_tm _ _ Eq_tm) s0)
+  end.
+Definition up_ren_ren_tm_tm {k : nat} {l : nat} {m : nat}
+  (xi : forall _ : fin k, fin l) (zeta : forall _ : fin l, fin m)
+  (rho : forall _ : fin k, fin m)
+  (Eq : forall x, eq (funcomp zeta xi x) (rho x)) :
+  forall x,
+  eq (funcomp (upRen_tm_tm zeta) (upRen_tm_tm xi) x) (upRen_tm_tm rho x) :=
+  up_ren_ren xi zeta rho Eq.
+Definition up_ren_ren_list_tm_tm {p : nat} {k : nat} {l : nat} {m : nat}
+  (xi : forall _ : fin k, fin l) (zeta : forall _ : fin l, fin m)
+  (rho : forall _ : fin k, fin m)
+  (Eq : forall x, eq (funcomp zeta xi x) (rho x)) :
+  forall x,
+  eq (funcomp (upRen_list_tm_tm p zeta) (upRen_list_tm_tm p xi) x)
+    (upRen_list_tm_tm p rho x) := up_ren_ren_p Eq.
+Fixpoint compRenRen_tm {k_tm : nat} {l_tm : nat} {m_tm : nat}
+(xi_tm : forall _ : fin m_tm, fin k_tm)
+(zeta_tm : forall _ : fin k_tm, fin l_tm)
+(rho_tm : forall _ : fin m_tm, fin l_tm)
+(Eq_tm : forall x, eq (funcomp zeta_tm xi_tm x) (rho_tm x)) (s : tm m_tm) :
+eq (ren_tm zeta_tm (ren_tm xi_tm s)) (ren_tm rho_tm s) :=
+  match s with
+  | var_tm _ s0 => ap (var_tm l_tm) (Eq_tm s0)
+  | app _ p s0 s1 =>
+      congr_app (compRenRen_tm xi_tm zeta_tm rho_tm Eq_tm s0)
+        (cod_comp (compRenRen_tm xi_tm zeta_tm rho_tm Eq_tm) s1)
+  | lam _ p s0 =>
+      congr_lam
+        (compRenRen_tm (upRen_list_tm_tm p xi_tm)
+           (upRen_list_tm_tm p zeta_tm) (upRen_list_tm_tm p rho_tm)
+           (up_ren_ren_p Eq_tm) s0)
+  end.
+Definition up_ren_subst_tm_tm {k : nat} {l : nat} {m_tm : nat}
+  (xi : forall _ : fin k, fin l) (tau : forall _ : fin l, tm m_tm)
+  (theta : forall _ : fin k, tm m_tm)
+  (Eq : forall x, eq (funcomp tau xi x) (theta x)) :
+  forall x, eq (funcomp (up_tm_tm tau) (upRen_tm_tm xi) x) (up_tm_tm theta x) :=
+  fun n =>
+  match n with
+  | Some fin_n => ap (ren_tm shift) (Eq fin_n)
+  | None => eq_refl
+  end.
+Definition up_ren_subst_list_tm_tm {p : nat} {k : nat} {l : nat} {m_tm : nat}
+  (xi : forall _ : fin k, fin l) (tau : forall _ : fin l, tm m_tm)
+  (theta : forall _ : fin k, tm m_tm)
+  (Eq : forall x, eq (funcomp tau xi x) (theta x)) :
+  forall x,
+  eq (funcomp (up_list_tm_tm p tau) (upRen_list_tm_tm p xi) x)
+    (up_list_tm_tm p theta x) :=
+  fun n =>
+  eq_trans (scons_p_comp' _ _ _ n)
+    (scons_p_congr (fun z => scons_p_head' _ _ z)
+       (fun z =>
+        eq_trans (scons_p_tail' _ _ (xi z)) (ap (ren_tm (shift_p p)) (Eq z)))).
+Fixpoint compRenSubst_tm {k_tm : nat} {l_tm : nat} {m_tm : nat}
+(xi_tm : forall _ : fin m_tm, fin k_tm)
+(tau_tm : forall _ : fin k_tm, tm l_tm)
+(theta_tm : forall _ : fin m_tm, tm l_tm)
+(Eq_tm : forall x, eq (funcomp tau_tm xi_tm x) (theta_tm x)) (s : tm m_tm) :
+eq (subst_tm tau_tm (ren_tm xi_tm s)) (subst_tm theta_tm s) :=
+  match s with
+  | var_tm _ s0 => Eq_tm s0
+  | app _ p s0 s1 =>
+      congr_app (compRenSubst_tm xi_tm tau_tm theta_tm Eq_tm s0)
+        (cod_comp (compRenSubst_tm xi_tm tau_tm theta_tm Eq_tm) s1)
+  | lam _ p s0 =>
+      congr_lam
+        (compRenSubst_tm (upRen_list_tm_tm p xi_tm) (up_list_tm_tm p tau_tm)
+           (up_list_tm_tm p theta_tm) (up_ren_subst_list_tm_tm _ _ _ Eq_tm)
+           s0)
+  end.
+Definition up_subst_ren_tm_tm {k : nat} {l_tm : nat} {m_tm : nat}
+  (sigma : forall _ : fin k, tm l_tm)
+  (zeta_tm : forall _ : fin l_tm, fin m_tm)
+  (theta : forall _ : fin k, tm m_tm)
+  (Eq : forall x, eq (funcomp (ren_tm zeta_tm) sigma x) (theta x)) :
+  forall x,
+  eq (funcomp (ren_tm (upRen_tm_tm zeta_tm)) (up_tm_tm sigma) x)
+    (up_tm_tm theta x) :=
+  fun n =>
+  match n with
+  | Some fin_n =>
+      eq_trans
+        (compRenRen_tm shift (upRen_tm_tm zeta_tm) (funcomp shift zeta_tm)
+           (fun x => eq_refl) (sigma fin_n))
+        (eq_trans
+           (eq_sym
+              (compRenRen_tm zeta_tm shift (funcomp shift zeta_tm)
+                 (fun x => eq_refl) (sigma fin_n)))
+           (ap (ren_tm shift) (Eq fin_n)))
+  | None => eq_refl
+  end.
+Definition up_subst_ren_list_tm_tm {p : nat} {k : nat} {l_tm : nat}
+  {m_tm : nat} (sigma : forall _ : fin k, tm l_tm)
+  (zeta_tm : forall _ : fin l_tm, fin m_tm)
+  (theta : forall _ : fin k, tm m_tm)
+  (Eq : forall x, eq (funcomp (ren_tm zeta_tm) sigma x) (theta x)) :
+  forall x,
+  eq
+    (funcomp (ren_tm (upRen_list_tm_tm p zeta_tm)) (up_list_tm_tm p sigma) x)
+    (up_list_tm_tm p theta x) :=
+  fun n =>
+  eq_trans (scons_p_comp' _ _ _ n)
+    (scons_p_congr (fun x => ap (var_tm (plus p m_tm)) (scons_p_head' _ _ x))
+       (fun n =>
+        eq_trans
+          (compRenRen_tm (shift_p p) (upRen_list_tm_tm p zeta_tm)
+             (funcomp (shift_p p) zeta_tm) (fun x => scons_p_tail' _ _ x)
+             (sigma n))
+          (eq_trans
+             (eq_sym
+                (compRenRen_tm zeta_tm (shift_p p)
+                   (funcomp (shift_p p) zeta_tm) (fun x => eq_refl) (sigma n)))
+             (ap (ren_tm (shift_p p)) (Eq n))))).
+Fixpoint compSubstRen_tm {k_tm : nat} {l_tm : nat} {m_tm : nat}
+(sigma_tm : forall _ : fin m_tm, tm k_tm)
+(zeta_tm : forall _ : fin k_tm, fin l_tm)
+(theta_tm : forall _ : fin m_tm, tm l_tm)
+(Eq_tm : forall x, eq (funcomp (ren_tm zeta_tm) sigma_tm x) (theta_tm x))
+(s : tm m_tm) :
+eq (ren_tm zeta_tm (subst_tm sigma_tm s)) (subst_tm theta_tm s) :=
+  match s with
+  | var_tm _ s0 => Eq_tm s0
+  | app _ p s0 s1 =>
+      congr_app (compSubstRen_tm sigma_tm zeta_tm theta_tm Eq_tm s0)
+        (cod_comp (compSubstRen_tm sigma_tm zeta_tm theta_tm Eq_tm) s1)
+  | lam _ p s0 =>
+      congr_lam
+        (compSubstRen_tm (up_list_tm_tm p sigma_tm)
+           (upRen_list_tm_tm p zeta_tm) (up_list_tm_tm p theta_tm)
+           (up_subst_ren_list_tm_tm _ _ _ Eq_tm) s0)
+  end.
+Definition up_subst_subst_tm_tm {k : nat} {l_tm : nat} {m_tm : nat}
+  (sigma : forall _ : fin k, tm l_tm) (tau_tm : forall _ : fin l_tm, tm m_tm)
+  (theta : forall _ : fin k, tm m_tm)
+  (Eq : forall x, eq (funcomp (subst_tm tau_tm) sigma x) (theta x)) :
+  forall x,
+  eq (funcomp (subst_tm (up_tm_tm tau_tm)) (up_tm_tm sigma) x)
+    (up_tm_tm theta x) :=
+  fun n =>
+  match n with
+  | Some fin_n =>
+      eq_trans
+        (compRenSubst_tm shift (up_tm_tm tau_tm)
+           (funcomp (up_tm_tm tau_tm) shift) (fun x => eq_refl) (sigma fin_n))
+        (eq_trans
+           (eq_sym
+              (compSubstRen_tm tau_tm shift (funcomp (ren_tm shift) tau_tm)
+                 (fun x => eq_refl) (sigma fin_n)))
+           (ap (ren_tm shift) (Eq fin_n)))
+  | None => eq_refl
+  end.
+Definition up_subst_subst_list_tm_tm {p : nat} {k : nat} {l_tm : nat}
+  {m_tm : nat} (sigma : forall _ : fin k, tm l_tm)
+  (tau_tm : forall _ : fin l_tm, tm m_tm) (theta : forall _ : fin k, tm m_tm)
+  (Eq : forall x, eq (funcomp (subst_tm tau_tm) sigma x) (theta x)) :
+  forall x,
+  eq (funcomp (subst_tm (up_list_tm_tm p tau_tm)) (up_list_tm_tm p sigma) x)
+    (up_list_tm_tm p theta x) :=
+  fun n =>
+  eq_trans (scons_p_comp' (funcomp (var_tm (plus p l_tm)) (zero_p p)) _ _ n)
+    (scons_p_congr
+       (fun x => scons_p_head' _ (fun z => ren_tm (shift_p p) _) x)
+       (fun n =>
+        eq_trans
+          (compRenSubst_tm (shift_p p) (up_list_tm_tm p tau_tm)
+             (funcomp (up_list_tm_tm p tau_tm) (shift_p p))
+             (fun x => eq_refl) (sigma n))
+          (eq_trans
+             (eq_sym
+                (compSubstRen_tm tau_tm (shift_p p) _
+                   (fun x => eq_sym (scons_p_tail' _ _ x)) (sigma n)))
+             (ap (ren_tm (shift_p p)) (Eq n))))).
+Fixpoint compSubstSubst_tm {k_tm : nat} {l_tm : nat} {m_tm : nat}
+(sigma_tm : forall _ : fin m_tm, tm k_tm)
+(tau_tm : forall _ : fin k_tm, tm l_tm)
+(theta_tm : forall _ : fin m_tm, tm l_tm)
+(Eq_tm : forall x, eq (funcomp (subst_tm tau_tm) sigma_tm x) (theta_tm x))
+(s : tm m_tm) :
+eq (subst_tm tau_tm (subst_tm sigma_tm s)) (subst_tm theta_tm s) :=
+  match s with
+  | var_tm _ s0 => Eq_tm s0
+  | app _ p s0 s1 =>
+      congr_app (compSubstSubst_tm sigma_tm tau_tm theta_tm Eq_tm s0)
+        (cod_comp (compSubstSubst_tm sigma_tm tau_tm theta_tm Eq_tm) s1)
+  | lam _ p s0 =>
+      congr_lam
+        (compSubstSubst_tm (up_list_tm_tm p sigma_tm)
+           (up_list_tm_tm p tau_tm) (up_list_tm_tm p theta_tm)
+           (up_subst_subst_list_tm_tm _ _ _ Eq_tm) s0)
+  end.
+Definition rinstInst_up_tm_tm {m : nat} {n_tm : nat}
+  (xi : forall _ : fin m, fin n_tm) (sigma : forall _ : fin m, tm n_tm)
+  (Eq : forall x, eq (funcomp (var_tm n_tm) xi x) (sigma x)) :
+  forall x,
+  eq (funcomp (var_tm (S n_tm)) (upRen_tm_tm xi) x) (up_tm_tm sigma x) :=
+  fun n =>
+  match n with
+  | Some fin_n => ap (ren_tm shift) (Eq fin_n)
+  | None => eq_refl
+  end.
+Definition rinstInst_up_list_tm_tm {p : nat} {m : nat} {n_tm : nat}
+  (xi : forall _ : fin m, fin n_tm) (sigma : forall _ : fin m, tm n_tm)
+  (Eq : forall x, eq (funcomp (var_tm n_tm) xi x) (sigma x)) :
+  forall x,
+  eq (funcomp (var_tm (plus p n_tm)) (upRen_list_tm_tm p xi) x)
+    (up_list_tm_tm p sigma x) :=
+  fun n =>
+  eq_trans (scons_p_comp' _ _ (var_tm (plus p n_tm)) n)
+    (scons_p_congr (fun z => eq_refl)
+       (fun n => ap (ren_tm (shift_p p)) (Eq n))).
+Fixpoint rinst_inst_tm {m_tm : nat} {n_tm : nat}
+(xi_tm : forall _ : fin m_tm, fin n_tm)
+(sigma_tm : forall _ : fin m_tm, tm n_tm)
+(Eq_tm : forall x, eq (funcomp (var_tm n_tm) xi_tm x) (sigma_tm x))
+(s : tm m_tm) : eq (ren_tm xi_tm s) (subst_tm sigma_tm s) :=
+  match s with
+  | var_tm _ s0 => Eq_tm s0
+  | app _ p s0 s1 =>
+      congr_app (rinst_inst_tm xi_tm sigma_tm Eq_tm s0)
+        (cod_ext (rinst_inst_tm xi_tm sigma_tm Eq_tm) s1)
+  | lam _ p s0 =>
+      congr_lam
+        (rinst_inst_tm (upRen_list_tm_tm p xi_tm) (up_list_tm_tm p sigma_tm)
+           (rinstInst_up_list_tm_tm _ _ Eq_tm) s0)
+  end.
+Lemma rinstInst_tm {m_tm : nat} {n_tm : nat}
+  (xi_tm : forall _ : fin m_tm, fin n_tm) :
+  eq (ren_tm xi_tm) (subst_tm (funcomp (var_tm n_tm) xi_tm)).
+Proof.
+exact (FunctionalExtensionality.functional_extensionality _ _
+                (fun x => rinst_inst_tm xi_tm _ (fun n => eq_refl) x)).
+Qed.
+Lemma instId_tm {m_tm : nat} : eq (subst_tm (var_tm m_tm)) id.
+Proof.
+exact (FunctionalExtensionality.functional_extensionality _ _
+                (fun x => idSubst_tm (var_tm m_tm) (fun n => eq_refl) (id x))).
+Qed.
+Lemma rinstId_tm {m_tm : nat} : eq (@ren_tm m_tm m_tm id) id.
+Proof.
+exact (eq_trans (rinstInst_tm (id _)) instId_tm).
+Qed.
+Lemma varL_tm {m_tm : nat} {n_tm : nat}
+  (sigma_tm : forall _ : fin m_tm, tm n_tm) :
+  eq (funcomp (subst_tm sigma_tm) (var_tm m_tm)) sigma_tm.
+Proof.
+exact (FunctionalExtensionality.functional_extensionality _ _
+                (fun x => eq_refl)).
+Qed.
+Lemma varLRen_tm {m_tm : nat} {n_tm : nat}
+  (xi_tm : forall _ : fin m_tm, fin n_tm) :
+  eq (funcomp (ren_tm xi_tm) (var_tm m_tm)) (funcomp (var_tm n_tm) xi_tm).
+Proof.
+exact (FunctionalExtensionality.functional_extensionality _ _
+                (fun x => eq_refl)).
+Qed.
+Lemma renRen_tm {k_tm : nat} {l_tm : nat} {m_tm : nat}
+  (xi_tm : forall _ : fin m_tm, fin k_tm)
+  (zeta_tm : forall _ : fin k_tm, fin l_tm) (s : tm m_tm) :
+  eq (ren_tm zeta_tm (ren_tm xi_tm s)) (ren_tm (funcomp zeta_tm xi_tm) s).
+Proof.
+exact (compRenRen_tm xi_tm zeta_tm _ (fun n => eq_refl) s).
+Qed.
+Lemma renRen'_tm {k_tm : nat} {l_tm : nat} {m_tm : nat}
+  (xi_tm : forall _ : fin m_tm, fin k_tm)
+  (zeta_tm : forall _ : fin k_tm, fin l_tm) :
+  eq (funcomp (ren_tm zeta_tm) (ren_tm xi_tm))
+    (ren_tm (funcomp zeta_tm xi_tm)).
+Proof.
+exact (FunctionalExtensionality.functional_extensionality _ _
+                (fun n => renRen_tm xi_tm zeta_tm n)).
+Qed.
+Lemma compRen_tm {k_tm : nat} {l_tm : nat} {m_tm : nat}
+  (sigma_tm : forall _ : fin m_tm, tm k_tm)
+  (zeta_tm : forall _ : fin k_tm, fin l_tm) (s : tm m_tm) :
+  eq (ren_tm zeta_tm (subst_tm sigma_tm s))
+    (subst_tm (funcomp (ren_tm zeta_tm) sigma_tm) s).
+Proof.
+exact (compSubstRen_tm sigma_tm zeta_tm _ (fun n => eq_refl) s).
+Qed.
+Lemma compRen'_tm {k_tm : nat} {l_tm : nat} {m_tm : nat}
+  (sigma_tm : forall _ : fin m_tm, tm k_tm)
+  (zeta_tm : forall _ : fin k_tm, fin l_tm) :
+  eq (funcomp (ren_tm zeta_tm) (subst_tm sigma_tm))
+    (subst_tm (funcomp (ren_tm zeta_tm) sigma_tm)).
+Proof.
+exact (FunctionalExtensionality.functional_extensionality _ _
+                (fun n => compRen_tm sigma_tm zeta_tm n)).
+Qed.
+Lemma renComp_tm {k_tm : nat} {l_tm : nat} {m_tm : nat}
+  (xi_tm : forall _ : fin m_tm, fin k_tm)
+  (tau_tm : forall _ : fin k_tm, tm l_tm) (s : tm m_tm) :
+  eq (subst_tm tau_tm (ren_tm xi_tm s)) (subst_tm (funcomp tau_tm xi_tm) s).
+Proof.
+exact (compRenSubst_tm xi_tm tau_tm _ (fun n => eq_refl) s).
+Qed.
+Lemma renComp'_tm {k_tm : nat} {l_tm : nat} {m_tm : nat}
+  (xi_tm : forall _ : fin m_tm, fin k_tm)
+  (tau_tm : forall _ : fin k_tm, tm l_tm) :
+  eq (funcomp (subst_tm tau_tm) (ren_tm xi_tm))
+    (subst_tm (funcomp tau_tm xi_tm)).
+Proof.
+exact (FunctionalExtensionality.functional_extensionality _ _
+                (fun n => renComp_tm xi_tm tau_tm n)).
+Qed.
+Lemma compComp_tm {k_tm : nat} {l_tm : nat} {m_tm : nat}
+  (sigma_tm : forall _ : fin m_tm, tm k_tm)
+  (tau_tm : forall _ : fin k_tm, tm l_tm) (s : tm m_tm) :
+  eq (subst_tm tau_tm (subst_tm sigma_tm s))
+    (subst_tm (funcomp (subst_tm tau_tm) sigma_tm) s).
+Proof.
+exact (compSubstSubst_tm sigma_tm tau_tm _ (fun n => eq_refl) s).
+Qed.
+Lemma compComp'_tm {k_tm : nat} {l_tm : nat} {m_tm : nat}
+  (sigma_tm : forall _ : fin m_tm, tm k_tm)
+  (tau_tm : forall _ : fin k_tm, tm l_tm) :
+  eq (funcomp (subst_tm tau_tm) (subst_tm sigma_tm))
+    (subst_tm (funcomp (subst_tm tau_tm) sigma_tm)).
+Proof.
+exact (FunctionalExtensionality.functional_extensionality _ _
+                (fun n => compComp_tm sigma_tm tau_tm n)).
+Qed.
+
+Arguments var_tm {n_tm}.
+
+Arguments app {n_tm}.
+
+Arguments lam {n_tm}.
+
+Global Instance Subst_tm { m_tm : nat } { n_tm : nat } : Subst1 ((fin) (m_tm) -> tm (n_tm)) (tm (m_tm)) (tm (n_tm)) := @subst_tm (m_tm) (n_tm) .
+
+Global Instance Ren_tm { m_tm : nat } { n_tm : nat } : Ren1 ((fin) (m_tm) -> (fin) (n_tm)) (tm (m_tm)) (tm (n_tm)) := @ren_tm (m_tm) (n_tm) .
+
+Global Instance VarInstance_tm { m_tm : nat } : Var ((fin) (m_tm)) (tm (m_tm)) := @var_tm (m_tm) .
+
+Notation "x '__tm'" := (var_tm x) (at level 5, format "x __tm") : subst_scope.
+
+Notation "x '__tm'" := (@ids (_) (_) VarInstance_tm x) (at level 5, only printing, format "x __tm") : subst_scope.
+
+Notation "'var'" := (var_tm) (only printing, at level 1) : subst_scope.
+
+Class Up_tm X Y := up_tm : X -> Y.
+
+Notation "↑__tm" := (up_tm) (only printing) : subst_scope.
+
+Notation "↑__tm" := (up_tm_tm) (only printing) : subst_scope.
+
+Global Instance Up_tm_tm { m : nat } { n_tm : nat } : Up_tm (_) (_) := @up_tm_tm (m) (n_tm) .
+
+Notation "s [ sigmatm ]" := (subst_tm sigmatm s) (at level 7, left associativity, only printing) : subst_scope.
+
+Notation "[ sigmatm ]" := (subst_tm sigmatm) (at level 1, left associativity, only printing) : fscope.
+
+Notation "s ⟨ xitm ⟩" := (ren_tm xitm s) (at level 7, left associativity, only printing) : subst_scope.
+
+Notation "⟨ xitm ⟩" := (ren_tm xitm) (at level 1, left associativity, only printing) : fscope.
+
+Ltac auto_unfold := repeat unfold subst1,  subst2,  Subst1,  Subst2,  ids,  ren1,  ren2,  Ren1,  Ren2,  Subst_tm,  Ren_tm,  VarInstance_tm.
+
+Tactic Notation "auto_unfold" "in" "*" := repeat unfold subst1,  subst2,  Subst1,  Subst2,  ids,  ren1,  ren2,  Ren1,  Ren2,  Subst_tm,  Ren_tm,  VarInstance_tm in *.
+
+Ltac asimpl' := repeat first [progress rewrite ?instId_tm| progress rewrite ?compComp_tm| progress rewrite ?compComp'_tm| progress rewrite ?rinstId_tm| progress rewrite ?compRen_tm| progress rewrite ?compRen'_tm| progress rewrite ?renComp_tm| progress rewrite ?renComp'_tm| progress rewrite ?renRen_tm| progress rewrite ?renRen'_tm| progress rewrite ?varL_tm| progress rewrite ?varLRen_tm| progress (unfold up_ren, upRen_tm_tm, upRen_list_tm_tm, up_tm_tm, up_list_tm_tm)| progress (cbn [subst_tm ren_tm])| fsimpl].
+
+Ltac asimpl := repeat try unfold_funcomp; auto_unfold in *; asimpl'; repeat try unfold_funcomp.
+
+Tactic Notation "asimpl" "in" hyp(J) := revert J; asimpl; intros J.
+
+Tactic Notation "auto_case" := auto_case (asimpl; cbn; eauto).
+
+Tactic Notation "asimpl" "in" "*" := auto_unfold in *; repeat first [progress rewrite ?instId_tm in *| progress rewrite ?compComp_tm in *| progress rewrite ?compComp'_tm in *| progress rewrite ?rinstId_tm in *| progress rewrite ?compRen_tm in *| progress rewrite ?compRen'_tm in *| progress rewrite ?renComp_tm in *| progress rewrite ?renComp'_tm in *| progress rewrite ?renRen_tm in *| progress rewrite ?renRen'_tm in *| progress rewrite ?varL_tm in *| progress rewrite ?varLRen_tm in *| progress (unfold up_ren, upRen_tm_tm, upRen_list_tm_tm, up_tm_tm, up_list_tm_tm in *)| progress (cbn [subst_tm ren_tm] in *)| fsimpl in *].
+
+Ltac substify := auto_unfold; try repeat (erewrite rinstInst_tm).
+
+Ltac renamify := auto_unfold; try repeat (erewrite <- rinstInst_tm).
