case-studies/kathrin/coq-submission/Chapter9/variadic_preservation.v
@@ -1,8 +1,6 @@
 (** ** Variadic Preservation *)
 
 Require Export ARS Program.Equality.
-Require Import core core_axioms fintype fintype_axioms.
-Import ScopedNotations.
 From Chapter6 Require Export variadic_fin.
 Set Implicit Arguments.
 Unset Strict Implicit.
