case-studies/kathrin/coq-submission/tactics.v
@@ -1,0 +1,30 @@
+Require Import header_extensible.
+
+(** ** Tactics for modular syntax  *)
+
+Ltac automate_inj :=
+repeat (match goal with
+  | [H : ?s = ?s |- _ ] => clear H
+  | [H : _ = _ |- _] => apply retract_inj in H; inversion H; subst
+  end).
+
+Hint Rewrite @retract_tight @retract_works: retract_forward.
+Hint Rewrite @retract_tight @retract_works : retract_rev.
+
+Class Imp X Y := imp:  X -> Y.
+Class ImpRev X Y := imprev:  X -> Y.
+
+Ltac msimpl := try reflexivity; repeat progress (first [ progress (autorewrite with retract_forward)  | cbn]).
+
+Ltac msimpl_in H := try apply retract_tight in H;
+                   try apply imprev in H;
+                   repeat progress (first [  progress (autorewrite with retract_rev in H) | cbn in H]).
+
+Ltac minversion H := msimpl_in H; try apply imprev in H; inversion H; repeat automate_inj; subst.
+Ltac induction_ H := msimpl_in H; try apply imprev in H; induction H; repeat automate_inj; subst.
+
+Ltac mconstructor := msimpl; try apply imprev; eapply imp; econstructor.
+
+Ltac mapply H := msimpl; try apply imprev; try (msimpl_in H);try (apply imprev in H);  eapply H.
+
+Ltac mapply_in H1 H2 := msimpl_in H1; try (msimpl_in H2); eapply H2 in H1.
